Gt3/HasTy/Nats.lean
@@ -1,0 +1,18 @@
+import Gt3.HasTy.Basic
+
+def Tm.ofNat {k} : ℕ → Tm k
+  | 0 => .zero
+  | n + 1 => .succ (.ofNat n)
+
+instance {k n} : OfNat (Tm k) n where ofNat := Tm.ofNat n
+
+theorem Tm.zero_def {k} : (0 : Tm k) = .zero := rfl
+
+theorem Ctx.HasTy.nat (n : ℕ) {Γ} (hΓ : Ok Γ) : HasTy Γ .nats (Tm.ofNat n) := by
+  induction n with | zero => exact zero hΓ | succ _ I => exact I.succ
+
+theorem Ctx.JEq.nat (n : ℕ) {Γ} (hΓ : Ok Γ) : JEq Γ .nats (Tm.ofNat n) (Tm.ofNat n)
+  := (HasTy.nat n hΓ).refl
+
+instance {k} : Add (Tm k) where
+  add a b := .natrec .nats (.succ (.bv 0)) a b
