Gt3/Syntax/Sugar.lean
@@ -1,0 +1,14 @@
+import Gt3.Syntax.Basic
+
+def Tm.wkn {k} (j : ℕ) : Tm k → Tm (k + 1)
+  | .fv x => .fv x
+  | .bv i => if i < j then .bv i.castSucc else .bv i.succ
+  | .univ ℓ => .univ ℓ
+
+-- def Tm.arr {k} (A B : Tm k) : Tm k := .pi A (↑₊B)
+
+-- @[simp]
+-- theorem Tm.open_arr {k} (A B : Tm (k + 1)) (x : String)
+-- : (Tm.arr A B).open x = .arr (A.open x) (B.open x) := by
+--   simp only [arr, open_pi]
+--   rw [B.open_castSucc]
